昔の証明を持ってきて改修してる

answer.v
@@ -468,7 +468,7 @@ case (f a) => /=.
 - by apply Nat.le_le_succ_r.
 Qed.
 
-(* Q10-2 *)
+(* Q10-3 *)
 Function quick_sort (xs: list nat) {measure length}: list nat :=
   match xs with
   | [] => []
@@ -486,37 +486,61 @@ Proof.
   by apply length_filter.
 Qed.
 
-(* Q10-3 *)
+(* Q10-4 *)
 Lemma quick_sort_nil : quick_sort nil = nil.
 Proof.
 by rewrite quick_sort_equation.
 Qed.
 
-(* Q10-4 *)
+(* Q10-5 *)
 Lemma quick_sort_single x1 : quick_sort [x1] = [x1].
 Proof.
 rewrite quick_sort_equation.
 by rewrite quick_sort_nil.
 Qed.
 
-(* Q10-5 *)
-Lemma filter_negb_In {A: Type}: forall xs (x: A) f g,
+(* Q10-6 *)
+Lemma filter_negb_In xs (x : nat) f g :
   In x xs ->
   (forall x', g x' = negb (f x')) ->
   In x (filter f xs) \/ In x (filter g xs).
 Proof.
-move => xs x f g Hxin.
+move => Hxin.
 case_eq (f x) => /= Hfx.
 - left.
   rewrite filter_In.
   by split.
 - right.
   rewrite filter_In.
-  split => //=.
+  split => //.
   by rewrite H Bool.negb_true_iff.
 Qed.
 
-(* Q10- *)
+(* Q10-7 *)
+Lemma sorted_app l r :
+  sorted l -> sorted r -> (forall lx rx, In lx l -> In rx r -> lx <= rx) ->
+  sorted (l ++ r).
+Proof.
+move => Hsorted_l Hsorted_r Hlx_le_rx.
+induction l as [ | n ] => //=.
+split.
+- move => x Hin_x.
+  rewrite in_app_iff in Hin_x.
+  case Hin_x.
+  + move => Hx_in.
+    rewrite /= in Hsorted_l.
+    case Hsorted_l => H _.
+    by apply H.
+  + apply Hlx_le_rx.
+    by apply in_eq.
+- apply IHl.
+  + by apply Hsorted_l.
+  + move => lx rx Hlx_in Hrx_in.
+    apply Hlx_le_rx => //=.
+    by right.
+Qed.
+
+(* Q10-8 *)
 Lemma quick_sort_In_ind xs x :
   (forall xs', length xs' < length xs -> (In x xs' <-> In x (quick_sort xs'))) ->
   (In x xs <-> In x (quick_sort xs)).
@@ -567,12 +591,155 @@ split => [ Hinx | ].
       by apply /le_lt_n_Sm /length_filter.
 Qed.
 
-(* Q10- *)
-Theorem quick_sort_sorted xs :
+Definition length_quick_sort_In(l: nat) :=
+  forall xs x, l = length xs -> In x xs <-> In x (quick_sort xs).
+
+(* Q10-9 *)
+Lemma quick_sort_In xs x :
+  In x xs <-> In x (quick_sort xs).
+Proof.
+apply (lt_wf_ind (length xs) length_quick_sort_In) => //.
+move => l Hlength_lt_In xs1 x1 Hxs1_length.
+subst.
+apply quick_sort_In_ind.
+move => xs2 Hxs2.
+by apply (Hlength_lt_In (length xs2)).
+Qed.
+
+(* Q10-10 *)
+Lemma quick_sort_sorted_length_ind xs :
+  (forall xs', length xs' < length xs -> sorted (quick_sort xs')) ->
   sorted (quick_sort xs).
 Proof.
-apply (lt_wf_ind (length xs) (fun len => forall xs, len = length xs -> sorted (quick_sort xs))) => //.
-move=> n Hind xs' Hlen.
+move=> Hsorted_quick_sort.
+case_eq xs. 
+  by rewrite quick_sort_nil.
+move=> x1 xs1 Hxs.
+rewrite quick_sort_equation.
+have: length xs = S (length xs1).
+  by rewrite Hxs /=.
+move=> Hxs_length.
+remember (quick_sort (filter (fun x : nat => x1 <=? x) xs1)) as right.
+case_eq (quick_sort (filter (fun x : nat => x <? x1) xs1)).
+- rewrite /=.
+  split.
+  + rewrite Heqright.
+    move=> x.
+    rewrite -quick_sort_In.
+    rewrite filter_In.
+    case.
+    move=> _.
+    by rewrite Nat.leb_le.
+  + rewrite Heqright.
+    apply Hsorted_quick_sort.
+    rewrite Hxs_length.
+    by apply /le_lt_n_Sm /length_filter.
+(* (head :: left) ++ x1 :: right *)
+- move=> head left Heqleft.
+  rewrite /=.
+  split.
+  + move=> x.
+    rewrite in_app_iff.
+    case.
+    * move=> Hinx_left.
+      suff: sorted (head :: left).
+        rewrite /=.
+        case.
+        move=> H _.
+        by apply (H x).
+      rewrite -Heqleft.
+      apply Hsorted_quick_sort.
+      rewrite Hxs_length.
+      by apply /le_lt_n_Sm /length_filter.
+    * move=> Hin_right.
+      have: x1 = x \/ In x right.
+        move: Hin_right.
+        by rewrite /=.
+      clear Hin_right.
+      have: In head (head :: left) -> head <= x1.
+        rewrite -Heqleft.
+        rewrite -quick_sort_In.
+        rewrite filter_In.
+        case => _.
+        rewrite ltb_lt.
+        by apply lt_le_incl.
+      move=> Hhead_le_x1.
+      case.
+      - move=> H; rewrite -H; clear H.
+        apply Hhead_le_x1.
+        apply in_eq.
+      - rewrite Heqright.
+        rewrite -quick_sort_In.
+        rewrite filter_In.
+        case => _.
+        rewrite Nat.leb_le.
+        apply Nat.le_trans.
+        apply Hhead_le_x1.
+        by apply in_eq.
+  + apply sorted_app.
+    * suff: sorted (head :: left).
+        rewrite /=.
+        by case.
+      rewrite -Heqleft.
+      apply: Hsorted_quick_sort.
+      rewrite Hxs_length.
+      by apply /le_lt_n_Sm /length_filter.
+    * rewrite Heqright.
+      rewrite /sorted -/sorted.
+      split.
+      - move=> x.
+        rewrite -quick_sort_In.
+        rewrite filter_In.
+        case.
+        by rewrite Nat.leb_le.
+      - apply: Hsorted_quick_sort.
+        rewrite Hxs_length.
+        by apply /le_lt_n_Sm /length_filter.
+    * move=> lx rx Hlx Hrx.
+      move: Nat.le_trans => H.
+      apply (H _ x1 _); clear H.
+      - suff: In lx (head :: left) -> lx <= x1.
+          apply.
+          rewrite /=.
+          by right.
+        rewrite -Heqleft.
+        rewrite -quick_sort_In.
+        rewrite filter_In.
+        case.
+        move=> _.
+        rewrite ltb_lt.
+        by apply lt_le_incl.
+      - move: Hrx.
+        rewrite /=.
+        case.
+          move=> H; by rewrite H.
+        rewrite Heqright.
+        rewrite -quick_sort_In.
+        rewrite filter_In.
+        case.
+        move=> _.
+        by rewrite leb_le.
+Qed.
+
+Definition length_quick_sort_sorted(l: nat) :=
+  forall xs, l = length xs -> sorted (quick_sort xs).
+
+(* Q10-11 *)
+Theorem quick_sort_sorted: forall xs,
+  sorted (quick_sort xs).
+Proof.
+move=> xs.
+apply (lt_wf_ind (length xs) length_quick_sort_sorted) => //.
+move=> len.
+rewrite /length_quick_sort_sorted.
+move=> Hlength_lt_sorted xs1 Hxs1_length.
+subst.
+apply quick_sort_sorted_length_ind.
+move=> xs2 Hxs2_length.
+apply (Hlength_lt_sorted (length xs2)) => //.
+Qed.
+
+
 
 
 
